verif_curve448Copy.v
@@ -1,0 +1,68 @@
+Require Import VST.floyd.proofauto.
+Require Import curve448.
+Require Import stdpp.list.
+Require Import ZArith.
+Require Import compcert.lib.Coqlib.
+
+Instance CompSpecs : compspecs. Proof. make_compspecs prog. Defined.
+Definition Vprog : varspecs.  mk_varspecs prog. Defined.
+
+Local Open Scope Z.
+
+Compute reptype (tarray tuint 14).
+Definition curve448Copy_spec : ident * funspec :=
+DECLARE _curve448Copy
+WITH  a : val, sha : share, contents_a : list val, (* Destination integer (editable) *)
+      b : val, contents_b : list Z,              (* Source integer *)
+      gv : globals
+PRE [ tptr tuint, tptr tuint ]
+    PROP   (writable_share sha;
+            Zlength contents_a = 14;
+            Zlength contents_b = 14)
+    PARAMS (a ; b) GLOBALS (gv)
+    SEP    (data_at sha (tarray tuint 14) contents_a a;
+            data_at Tsh (tarray tuint 14) (map Vint (map Int.repr (contents_b))) b)
+POST [ tvoid ]
+    PROP   ()
+    RETURN ()
+    SEP    (data_at sha (tarray tuint 14) (map Vint (map Int.repr (contents_b))) a;
+            data_at Tsh (tarray tuint 14) (map Vint (map Int.repr (contents_b))) b).
+
+Definition curve448Copy_INV a sha contents_a b contents_b := 
+   (EX i : Z,
+   (PROP   (writable_share sha; 
+            Zlength contents_a = 14;
+            Zlength contents_b = 14)
+   LOCAL   (temp _a a; temp _b b)
+   SEP     (data_at sha (tarray tuint 14) 
+               (  sublist.sublist 0 i (map Vint (map Int.repr (contents_b))) 
+               ++ sublist.sublist i 14 contents_a) a ;
+            data_at Tsh (tarray tuint 14) (map Vint (map Int.repr (contents_b))) b
+            )))%assert.
+
+Definition Gprog : funspecs := ltac:(with_library prog [ curve448Copy_spec ]).
+
+Lemma body_curve448SetInt : semax_body Vprog Gprog f_curve448Copy curve448Copy_spec.
+Proof.
+(* Initialize everything. *)
+start_function. 
+(* Get loop started. *)
+forward_for_simple_bound 14 (curve448Copy_INV a sha contents_a b contents_b).
+(* Show PRE implies INV. *)
+entailer!.
+autorewrite with sublist.
+list_simplify.
+
+(* Step through loop. *)
+forward.
+forward.
+(* Show INV is actually INV as the loop happens. *)
+entailer!.
+autorewrite with sublist.
+list_simplify.
+
+(* Show INV implies POST. *)
+entailer!.
+autorewrite with sublist.
+list_simplify.
+Qed.
