verif_curve448Swap.v
@@ -1,0 +1,126 @@
+Require Import VST.floyd.proofauto.
+Require Import curve448.
+Require Import stdpp.list.
+Require Import ZArith.
+Require Import compcert.lib.Coqlib.
+
+(* /**
+ * @brief Conditional swap
+ * @param[in,out] a Pointer to the first integer
+ * @param[in,out] b Pointer to the second integer
+ * @param[in] c Condition variable
+ **/
+
+void curve448Swap(uint32_t *a, uint32_t *b, uint32_t c)
+{
+   uint_t i;
+   uint32_t mask;
+   uint32_t dummy;
+
+   //The mask is the all-1 or all-0 word
+   mask = ~c + 1;
+
+   //Conditional swap
+   for(i = 0; i < 14; i++)
+   {
+      //Constant time implementation
+      dummy = mask & (a[i] ^ b[i]);
+      a[i] ^= dummy;
+      b[i] ^= dummy;
+   }
+}
+*)
+
+Instance CompSpecs : compspecs. Proof. make_compspecs prog. Defined.
+Definition Vprog : varspecs.  mk_varspecs prog. Defined.
+
+Local Open Scope Z.
+
+Scheme Equality for list.
+
+Definition curve448Swap_spec : ident * funspec :=
+DECLARE _curve448Swap
+WITH a : val, sha : share, contents_a : list Z,
+     b : val, shb : share, contents_b : list Z,
+     c : Z, (* Should be 0 or 1. See PROP in PRE.  *)
+     gv : globals
+PRE [ tptr tuint, tptr tuint, tuint ]
+    PROP   (writable_share sha; 
+            writable_share shb;
+            Zlength contents_a = 14;
+            Zlength contents_b = 14;
+            c = 0 \/ c = 1)
+    PARAMS ( a ; b ; Vint(Int.repr c)) GLOBALS (gv)
+    SEP    (data_at sha (tarray tuint 14) (map Vint (map Int.repr contents_a)) a;
+            data_at shb (tarray tuint 14) (map Vint (map Int.repr contents_b)) b)
+POST [ tvoid ]
+    PROP   ()
+    RETURN ()
+    SEP    (data_at sha (tarray tuint 14) 
+                (if (Z.eqb c 0) then (map Vint (map Int.repr contents_a))
+                 else map Vint (map Int.repr contents_b)) a;
+            data_at shb (tarray tuint 14) 
+                (if (Z.eqb c 0) then (map Vint (map Int.repr contents_b))
+                else map Vint (map Int.repr contents_a)) b). 
+            (* If c = 0, no swap. Else, swap. *)
+
+Definition curve448Swap_INV a contents_a b contents_b c:=
+(EX i : Z,
+(PROP   (Zlength contents_a = 14;
+         Zlength contents_b = 14)
+LOCAL   (temp _a a; temp _b b; temp _mask (Vint (Int.repr (((c + 1) mod 2) - 1))))
+SEP     ( (* What is the loop invariant? 
+                Idea: 
+                 If c = 0, then a = a and b = b.
+                 If c = 1, then a and b are partially swapped up to index i. *)
+         data_at Tsh (tarray tuint 14) (map Vint (map Int.repr contents_a)) a;
+         data_at Tsh (tarray tuint 14) (map Vint (map Int.repr contents_b)) b
+        )))%assert.
+
+
+(* TESTING THIS IN C COMPILER:
+
+#include <stdio.h>
+/**
+ * @brief Conditional swap
+ * @param[in,out] a Pointer to the first integer
+ * @param[in,out] b Pointer to the second integer
+ * @param[in] c Condition variable
+ **/
+
+typedef unsigned long uint32_t;
+typedef unsigned int uint_t;
+const int size = 2;
+void curve448Swap(int *a, int *b, uint32_t c)
+{
+   uint_t i;
+   uint32_t mask;
+   uint32_t dummy;
+
+   //The mask is the all-1 or all-0 word
+   mask = ~c + 1;
+
+   //Conditional swap
+   for(i = 0; i < size; i++)
+   {
+      //Constant time implementation
+      dummy = mask & (a[i] ^ b[i]);
+      a[i] ^= dummy;
+      b[i] ^= dummy;
+   }
+}
+int main() {
+int a[2] = {1, 2};
+int b[2] = {3, 4};
+
+curve448Swap(a,b,1);
+
+printf("a:");
+int i;
+for(i=0; i < size; i++)
+{
+    printf("%d, ", a[i]);
+}
+
+}
+*)
